P2st new invariant proof done

examples/ProcTwoStInv.v
@@ -34,7 +34,7 @@ Section Invariants.
                                 getStAddr getStSrc calcStAddr getStVSrc
                                 getSrc1 execState execNextPc.
 
-  Definition p2st_pc_epochs_inv
+  Definition p2st_pc_epochs_inv_body
              (fepochv eepochv d2efullv e2dfullv stallv: fullType type (SyntaxKind Bool))
              (pcv: fullType type (SyntaxKind (Bit addrSize)))
              (d2eeltv stalledv: fullType type (SyntaxKind (d2eElt addrSize lgDataBytes rfIdx))) :=
@@ -52,7 +52,32 @@ Section Invariants.
     (stallv = true -> d2efullv = false -> e2dfullv = false ->
      stalledv ``"nextPc" = pcv).
 
-  Definition p2st_decode_inv
+  Record p2st_pc_epochs_inv (o: RegsT) : Prop :=
+    { pcv0 : fullType type (SyntaxKind (Bit addrSize));
+      Hpcv0 : M.find "pc"%string o = Some (existT _ _ pcv0);
+      fepochv0 : fullType type (SyntaxKind Bool);
+      Hfepochv0 : M.find "fEpoch"%string o = Some (existT _ _ fepochv0);
+
+      d2eeltv0 : fullType type (SyntaxKind (d2eElt addrSize lgDataBytes rfIdx));
+      Hd2eeltv0 : M.find "d2e"--"elt"%string o = Some (existT _ _ d2eeltv0);
+      d2efullv0 : fullType type (SyntaxKind Bool);
+      Hd2efullv0 : M.find "d2e"--"full"%string o = Some (existT _ _ d2efullv0);
+      e2dfullv0 : fullType type (SyntaxKind Bool);
+      He2dfullv0 : M.find "e2d"--"full"%string o = Some (existT _ _ e2dfullv0);
+
+      stallv0 : fullType type (SyntaxKind Bool);
+      Hstallv0 : M.find "stall"%string o = Some (existT _ _ stallv0);
+      stalledv0 : fullType type (SyntaxKind (d2eElt addrSize lgDataBytes rfIdx));
+      Hstalledv0 : M.find "stalled"%string o = Some (existT _ _ stalledv0);
+
+      eepochv0 : fullType type (SyntaxKind Bool);
+      Heepochv0 : M.find "eEpoch"%string o = Some (existT _ _ eepochv0);
+    
+      Hinv0 : p2st_pc_epochs_inv_body fepochv0 eepochv0 d2efullv0 e2dfullv0
+                                      stallv0 pcv0 d2eeltv0 stalledv0 }.
+
+  (* NOTE: this invariant requires p2st_raw_inv *)
+  Definition p2st_decode_inv_body
              (pgmv: fullType type (SyntaxKind (Vector (Data lgDataBytes) addrSize)))
              (rfv: fullType type (SyntaxKind (Vector (Data lgDataBytes) rfIdx)))
              (d2efullv: fullType type (SyntaxKind Bool))
@@ -74,71 +99,80 @@ Section Invariants.
     (d2eeltv ``"opType" = opTh ->
      d2eeltv ``"val" = rfv (evalExpr (getSrc1 _ rawInst))).
 
-  Definition p2st_raw_inv
+  Record p2st_decode_inv (o: RegsT) : Prop :=
+    { pgmv1 : fullType type (SyntaxKind (Vector (Data lgDataBytes) addrSize));
+      Hpgmv1 : M.find "pgm"%string o = Some (existT _ _ pgmv1);
+
+      rfv1 : fullType type (SyntaxKind (Vector (Data lgDataBytes) rfIdx));
+      Hrfv1 : M.find "rf"%string o = Some (existT _ _ rfv1);
+
+      d2eeltv1 : fullType type (SyntaxKind (d2eElt addrSize lgDataBytes rfIdx));
+      Hd2eeltv1 : M.find "d2e"--"elt"%string o = Some (existT _ _ d2eeltv1);
+      d2efullv1 : fullType type (SyntaxKind Bool);
+      Hd2efullv1 : M.find "d2e"--"full"%string o = Some (existT _ _ d2efullv1);
+
+      Hinv1 : p2st_decode_inv_body pgmv1 rfv1 d2efullv1 d2eeltv1 }.
+
+  (* NOTE: this invariant requires p2st_scoreboard_inv *)
+  Definition p2st_raw_inv_body
              (d2efullv stallv: fullType type (SyntaxKind Bool))
              (d2eeltv stalledv: fullType type (SyntaxKind (d2eElt addrSize lgDataBytes rfIdx))) :=
     d2efullv = true -> stallv = true -> stalledv ``"opType" = opLd ->
-    (d2eeltv ``"opType" = opSt ->
-     (stalledv ``"dst" <> evalExpr (getStSrc _ (d2eeltv ``"rawInst")) /\
-      stalledv ``"dst" <> evalExpr (getStVSrc _ (d2eeltv ``"rawInst")))) /\
-    (d2eeltv ``"opType" = opLd ->
-     stalledv ``"dst" <> evalExpr (getLdSrc _ (d2eeltv ``"rawInst"))) /\
-    (d2eeltv ``"opType" = opTh ->
-     stalledv ``"dst" <> evalExpr (getSrc1 _ (d2eeltv ``"rawInst"))).
+    ((d2eeltv ``"opType" = opSt ->
+      (stalledv ``"dst" <> evalExpr (getStSrc _ (d2eeltv ``"rawInst")) /\
+       stalledv ``"dst" <> evalExpr (getStVSrc _ (d2eeltv ``"rawInst")))) /\
+     (d2eeltv ``"opType" = opLd ->
+      stalledv ``"dst" <> evalExpr (getLdSrc _ (d2eeltv ``"rawInst"))) /\
+     (d2eeltv ``"opType" = opTh ->
+      stalledv ``"dst" <> evalExpr (getSrc1 _ (d2eeltv ``"rawInst")))).
 
-  Definition p2st_scoreboard_inv
+  Record p2st_raw_inv (o: RegsT) : Prop :=
+    { d2eeltv2 : fullType type (SyntaxKind (d2eElt addrSize lgDataBytes rfIdx));
+      Hd2eeltv2 : M.find "d2e"--"elt"%string o = Some (existT _ _ d2eeltv2);
+      d2efullv2 : fullType type (SyntaxKind Bool);
+      Hd2efullv2 : M.find "d2e"--"full"%string o = Some (existT _ _ d2efullv2);
+
+      stallv2 : fullType type (SyntaxKind Bool);
+      Hstallv2 : M.find "stall"%string o = Some (existT _ _ stallv2);
+      stalledv2 : fullType type (SyntaxKind (d2eElt addrSize lgDataBytes rfIdx));
+      Hstalledv2 : M.find "stalled"%string o = Some (existT _ _ stalledv2);
+
+      Hinv : p2st_raw_inv_body d2efullv2 stallv2 d2eeltv2 stalledv2 }.
+
+  Definition p2st_scoreboard_inv_body
              (d2efullv stallv sbvv: fullType type (SyntaxKind Bool))
              (sbv: fullType type (SyntaxKind (Bit rfIdx)))
              (d2eeltv stalledv: fullType type (SyntaxKind (d2eElt addrSize lgDataBytes rfIdx))) :=
-    (d2efullv = false -> stallv = true -> sbvv = true /\ stalledv ``"dst" = sbv) /\
-    (d2efullv = true -> d2eeltv ``"opType" = opLd -> sbvv = true /\ d2eeltv ``"dst" = sbv).
-  
-  Record p2st_inv (o: RegsT) : Prop :=
-    { pcv : fullType type (SyntaxKind (Bit addrSize));
-      Hpcv : M.find "pc"%string o = Some (existT _ _ pcv);
-      pgmv : fullType type (SyntaxKind (Vector (Data lgDataBytes) addrSize));
-      Hpgmv : M.find "pgm"%string o = Some (existT _ _ pgmv);
-      fepochv : fullType type (SyntaxKind Bool);
-      Hfepochv : M.find "fEpoch"%string o = Some (existT _ _ fepochv);
+    stallv = true -> stalledv ``"opType" = opLd -> (sbvv = true /\ stalledv ``"dst" = sbv).
 
-      rfv : fullType type (SyntaxKind (Vector (Data lgDataBytes) rfIdx));
-      Hrfv : M.find "rf"%string o = Some (existT _ _ rfv);
+  Record p2st_scoreboard_inv (o: RegsT) : Prop :=
+    { sbv3 : fullType type (SyntaxKind (Bit rfIdx));
+      Hsbv3 : M.find "idx"%string o = Some (existT _ _ sbv3);
+      sbvv3 : fullType type (SyntaxKind Bool);
+      Hsbvv3 : M.find "valid"%string o = Some (existT _ _ sbvv3);
 
-      sbv : fullType type (SyntaxKind (Bit rfIdx));
-      Hsbv : M.find "idx"%string o = Some (existT _ _ sbv);
-      sbvv : fullType type (SyntaxKind Bool);
-      Hsbvv : M.find "valid"%string o = Some (existT _ _ sbvv);
+      d2eeltv3 : fullType type (SyntaxKind (d2eElt addrSize lgDataBytes rfIdx));
+      Hd2eeltv3 : M.find "d2e"--"elt"%string o = Some (existT _ _ d2eeltv3);
+      d2efullv3 : fullType type (SyntaxKind Bool);
+      Hd2efullv3 : M.find "d2e"--"full"%string o = Some (existT _ _ d2efullv3);
 
-      d2eeltv : fullType type (SyntaxKind (d2eElt addrSize lgDataBytes rfIdx));
-      Hd2eeltv : M.find "d2e"--"elt"%string o = Some (existT _ _ d2eeltv);
-      d2efullv : fullType type (SyntaxKind Bool);
-      Hd2efullv : M.find "d2e"--"full"%string o = Some (existT _ _ d2efullv);
+      stallv3 : fullType type (SyntaxKind Bool);
+      Hstallv3 : M.find "stall"%string o = Some (existT _ _ stallv3);
+      stalledv3 : fullType type (SyntaxKind (d2eElt addrSize lgDataBytes rfIdx));
+      Hstalledv3 : M.find "stalled"%string o = Some (existT _ _ stalledv3);
 
-      e2deltv : fullType type (SyntaxKind (Bit addrSize));
-      He2deltv : M.find "e2d"--"elt"%string o = Some (existT _ _ e2deltv);
-      e2dfullv : fullType type (SyntaxKind Bool);
-      He2dfullv : M.find "e2d"--"full"%string o = Some (existT _ _ e2dfullv);
+      Hinv : p2st_scoreboard_inv_body d2efullv3 stallv3 sbvv3 sbv3 d2eeltv3 stalledv3 }.
 
-      stallv : fullType type (SyntaxKind Bool);
-      Hstallv : M.find "stall"%string o = Some (existT _ _ stallv);
-      stalledv : fullType type (SyntaxKind (d2eElt addrSize lgDataBytes rfIdx));
-      Hstalledv : M.find "stalled"%string o = Some (existT _ _ stalledv);
+  Hint Unfold p2st_pc_epochs_inv_body p2st_decode_inv_body
+       p2st_raw_inv_body p2st_scoreboard_inv_body : InvDefs.
 
-      eepochv : fullType type (SyntaxKind Bool);
-      Heepochv : M.find "eEpoch"%string o = Some (existT _ _ eepochv);
-
-      Hinv :
-        p2st_pc_epochs_inv fepochv eepochv d2efullv e2dfullv stallv pcv d2eeltv stalledv
-        (* p2st_decode_inv pgmv rfv d2efullv d2eeltv /\ *)
-        (* p2st_raw_inv d2efullv stallv d2eeltv stalledv /\ *)
-        (* p2st_scoreboard_inv d2efullv stallv sbvv sbv d2eeltv stalledv *)
-    }.
-  Hint Unfold p2st_pc_epochs_inv p2st_decode_inv p2st_raw_inv p2st_scoreboard_inv: InvDefs.
-  
   Ltac p2st_inv_old :=
-    try match goal with
-        | [H: p2st_inv _ |- _] => destruct H
-        end;
+    repeat match goal with
+           | [H: p2st_pc_epochs_inv _ |- _] => destruct H
+           | [H: p2st_decode_inv _ |- _] => destruct H
+           | [H: p2st_raw_inv _ |- _] => destruct H
+           | [H: p2st_scoreboard_inv _ |- _] => destruct H
+           end;
     kinv_red.
 
   Ltac p2st_inv_new :=
@@ -155,13 +189,126 @@ Section Invariants.
 
   Ltac p2st_inv_tac := p2st_inv_old; p2st_inv_new.
 
-  Lemma p2st_inv_ok':
+  Lemma p2st_scoreboard_inv_ok':
     forall init n ll,
       init = initRegs (getRegInits (fst p2stInl)) ->
       Multistep (fst p2stInl) init n ll ->
-      p2st_inv n.
+      p2st_scoreboard_inv n.
   Proof. (* SKIP_PROOF_ON
     induction 2.
+
+    - p2st_inv_old.
+      unfold getRegInits, fst, p2stInl, ProcTwoStInl.p2stInl.
+      p2st_inv_new; simpl in *; kinv_simpl.
+
+    - kinvert.
+      + mred.
+      + mred.
+      + kinv_dest_custom p2st_inv_tac.
+      + kinv_dest_custom p2st_inv_tac.
+      + kinv_dest_custom p2st_inv_tac.
+      + kinv_dest_custom p2st_inv_tac.
+      + kinv_dest_custom p2st_inv_tac.
+      + kinv_dest_custom p2st_inv_tac.
+      + kinv_dest_custom p2st_inv_tac.
+      + kinv_dest_custom p2st_inv_tac.
+      + kinv_dest_custom p2st_inv_tac;
+          try (match goal with
+               | [H1: ?x ?s1 = _, H2: ?x ?s2 = _ |- _] => change s1 with s2 in H1
+               end; rewrite e in H2; inv H2).
+      + kinv_dest_custom p2st_inv_tac.
+      + kinv_dest_custom p2st_inv_tac.
+      + kinv_dest_custom p2st_inv_tac.
+      + kinv_dest_custom p2st_inv_tac.
+
+        END_SKIP_PROOF_ON *) admit.
+  Qed.
+
+  Lemma p2st_raw_inv_ok':
+    forall init n ll,
+      init = initRegs (getRegInits (fst p2stInl)) ->
+      Multistep (fst p2stInl) init n ll ->
+      p2st_raw_inv n.
+  Proof. (* SKIP_PROOF_ON
+    induction 2; intros.
+
+    - p2st_inv_old.
+      unfold getRegInits, fst, p2stInl, ProcTwoStInl.p2stInl.
+      p2st_inv_new; simpl in *; kinv_simpl.
+
+    - pose proof (p2st_scoreboard_inv_ok' H H0).
+      kinvert.
+      + mred.
+      + mred.
+      + kinv_dest_custom p2st_inv_tac.
+      + kinv_dest_custom p2st_inv_tac; try (rewrite e in H5; inv H5; fail).
+        rewrite andb_true_l in H15; kinv_simpl; intuition idtac.
+      + kinv_dest_custom p2st_inv_tac; try (rewrite e in H7; inv H7; fail).
+        * rewrite andb_true_l in H4; kinv_simpl; intuition idtac.
+        * rewrite andb_true_l in H12; kinv_simpl; intuition idtac.
+      + kinv_dest_custom p2st_inv_tac; try (rewrite e in H5; inv H5; fail).
+        rewrite andb_true_l in H15; kinv_simpl; intuition idtac.
+      + kinv_dest_custom p2st_inv_tac; try (rewrite e in H7; inv H7; fail).
+      + kinv_dest_custom p2st_inv_tac.
+      + kinv_dest_custom p2st_inv_tac.
+      + kinv_dest_custom p2st_inv_tac.
+      + kinv_dest_custom p2st_inv_tac.
+      + kinv_dest_custom p2st_inv_tac.
+      + kinv_dest_custom p2st_inv_tac.
+      + kinv_dest_custom p2st_inv_tac.
+      + kinv_dest_custom p2st_inv_tac.
+
+        END_SKIP_PROOF_ON *) admit.
+  Qed.
+
+  Lemma p2st_decode_inv_ok':
+    forall init n ll,
+      init = initRegs (getRegInits (fst p2stInl)) ->
+      Multistep (fst p2stInl) init n ll ->
+      p2st_decode_inv n.
+  Proof. (* SKIP_PROOF_ON
+    induction 2; intros.
+
+    - p2st_inv_old.
+      unfold getRegInits, fst, p2stInl, ProcTwoStInl.p2stInl.
+      p2st_inv_new; simpl in *; kinv_simpl.
+
+    - pose proof (p2st_raw_inv_ok' H H0).
+      kinvert.
+      + mred.
+      + mred.
+      + kinv_dest_custom p2st_inv_tac.
+      + kinv_dest_custom p2st_inv_tac; try (rewrite e in H1; inv H1; fail).
+      + kinv_dest_custom p2st_inv_tac; try (rewrite e in H1; inv H1; fail).
+      + kinv_dest_custom p2st_inv_tac; try (rewrite e in H1; inv H1; fail).
+      + kinv_dest_custom p2st_inv_tac; try (rewrite e in H1; inv H1; fail).
+      + kinv_dest_custom p2st_inv_tac.
+      + kinv_dest_custom p2st_inv_tac.
+      + kinv_dest_custom p2st_inv_tac.
+      + kinv_dest_custom p2st_inv_tac.
+      + kinv_dest_custom p2st_inv_tac.
+        * find_if_inside; [elim H15; auto|auto].
+        * find_if_inside; [elim H9; auto|auto].
+        * find_if_inside; [elim H17; auto|auto].
+        * find_if_inside; [elim H7; auto|auto].
+        * find_if_inside; [elim H15; auto|auto].
+        * find_if_inside; [elim H9; auto|auto].
+        * find_if_inside; [elim H17; auto|auto].
+        * find_if_inside; [elim H7; auto|auto].
+      + kinv_dest_custom p2st_inv_tac.
+      + kinv_dest_custom p2st_inv_tac.
+      + kinv_dest_custom p2st_inv_tac.
+
+        END_SKIP_PROOF_ON *) admit.
+  Qed.
+
+  Lemma p2st_pc_epochs_inv_ok':
+    forall init n ll,
+      init = initRegs (getRegInits (fst p2stInl)) ->
+      Multistep (fst p2stInl) init n ll ->
+      p2st_pc_epochs_inv n.
+  Proof. (* SKIP_PROOF_ON
+    induction 2; intros.
 
     - p2st_inv_old.
       unfold getRegInits, fst, p2stInl, ProcTwoStInl.p2stInl.
@@ -192,13 +339,20 @@ Section Invariants.
   Lemma p2st_inv_ok:
     forall o,
       reachable o (fst p2stInl) ->
-      p2st_inv o.
+      p2st_pc_epochs_inv o /\ p2st_decode_inv o /\
+      p2st_raw_inv o /\ p2st_scoreboard_inv o.
   Proof.
     intros; inv H; inv H0.
-    eapply p2st_inv_ok'; eauto.
+    repeat split.
+    - eapply p2st_pc_epochs_inv_ok'; eauto.
+    - eapply p2st_decode_inv_ok'; eauto.
+    - eapply p2st_raw_inv_ok'; eauto.
+    - eapply p2st_scoreboard_inv_ok'; eauto.
   Qed.
 
 End Invariants.
 
 Hint Unfold RqFromProc RsToProc: MethDefs.
+Hint Unfold p2st_pc_epochs_inv_body p2st_decode_inv_body
+     p2st_raw_inv_body p2st_scoreboard_inv_body : InvDefs.
 
